CBPV/Syntax.lean
@@ -162,10 +162,7 @@ def renameValComp ξ ζ v : renameVal ξ (renameVal ζ v) = renameVal (ξ ∘ ζ
 def renameComComp ξ ζ m : renameCom ξ (renameCom ζ m) = renameCom (ξ ∘ ζ) m :=
   (renameComp ξ ζ (ξ ∘ ζ) (λ _ ↦ rfl)).right m
 
-/-*------------------------------
-  Applying join point renamings
-------------------------------*-/
-
+-- Join point renamings
 @[simp]
 def renameJCom (ξ : Nat → Nat) : Com → Com
   | letin m n => letin m (renameJCom ξ n)
@@ -173,17 +170,6 @@ def renameJCom (ξ : Nat → Nat) : Com → Com
   | join n m => join (renameJCom ξ n) (renameJCom (lift ξ) m)
   | jump j v => jump (ξ j) v
   | m => m
-
-theorem renameJComExt ξ ζ (h : ∀ x, ξ x = ζ x) : ∀ m, renameJCom ξ m = renameJCom ζ m := by
-  intro m; mutual_induction m generalizing ξ ζ
-  all_goals simp; try repeat' constructor
-  all_goals apply_rules [liftExt]
-
-theorem renameJComId : ∀ m, renameJCom id m = m := by
-  intro m; mutual_induction m
-  all_goals simp; try constructor
-  all_goals try assumption
-  case join ih => rw [renameJComExt (lift id) id (liftId _ (λ _ ↦ rfl))]; exact ih
 
 /-*----------------------
   Lifting substitutions
@@ -498,24 +484,3 @@ theorem wRenameLift {ξ : Nat → Nat} {Γ Δ A}
   cases mem with
   | here => exact In.here
   | there => apply_rules [In.there]
-
-/-*---------------------------------
-  Well-scoped join point renamings
----------------------------------*-/
-
-def wRenameJ (ξ : Nat → Nat) (Δ Φ : Dtxt) := ∀ j A B, Δ ∋ j ∶ A ↗ B → Φ ∋ ξ j ∶ A ↗ B
-notation:40 Φ:41 "⊢" ξ:41 "∶" Δ:41 => wRenameJ ξ Δ Φ
-
-theorem wRenameJSucc {Δ A B} : Δ ∷ A ↗ B ⊢ succ ∶ Δ := by
-  intro x A B mem; constructor; assumption
-
-theorem wRenameJLift {ξ : Nat → Nat} {Δ Φ : Dtxt} {A B}
-  (h : Φ ⊢ ξ ∶ Δ) :
-  Φ ∷ A ↗ B ⊢ lift ξ ∶ Δ ∷ A ↗ B := by
-  intro x A B mem
-  cases mem with
-  | here => exact Jn.here
-  | there => apply_rules [Jn.there]
-
-theorem wRenameJNil {Δ : Dtxt} : Δ ⊢ id ∶ ⬝ := by
-  intro x A B mem; cases mem
